Define WP in terms of WPC (leaving many things broken)

src/high/crash_weakestpre.v
@@ -1,12 +1,136 @@
 From iris.proofmode Require Import base tactics classes.
+From iris.algebra Require Import agree auth.
+From Perennial.base_logic.lib Require Export ncfupd.
 From Perennial.program_logic Require crash_weakestpre.
 
 From self.high Require Export dprop.
 From self.base Require Import primitive_laws.
-From self.high Require Import weakestpre.
+From self.high Require Import resources.
+
+(** We define a few things about the resource algebra that that we use to encode
+abstract histories. *)
+Section abs_history_lemmas.
+  Context `{hG : nvmG Σ}.
+  Context `{Countable ST}.
+
+  Implicit Types (abs_hist : abs_history ST) (ℓ : loc).
+
+  Definition abs_hist_to_ra abs_hist : encoded_abs_historyR :=
+    (to_agree ∘ encode) <$> abs_hist.
+
+  Definition own_full_history (abs_hists : gmap loc (gmap time positive)) :=
+    own abs_history_name ((● ((λ h, ● (to_agree <$> h)) <$> abs_hists)) : abs_historiesR).
+
+  Definition know_full_history_loc ℓ abs_hist :=
+    own abs_history_name ((◯ {[ ℓ := ● (abs_hist_to_ra abs_hist) ]}) : abs_historiesR).
+
+  Definition know_full_encoded_history_loc ℓ (abs_hist : gmap time st) :=
+    own abs_history_name ((◯ {[ ℓ := ● ((to_agree <$> abs_hist) : gmap _ (agreeR stO)) ]}) : abs_historiesR).
+
+  Definition know_frag_history_loc ℓ abs_hist :=
+    own abs_history_name ((◯ {[ ℓ := ◯ (abs_hist_to_ra abs_hist) ]}) : abs_historiesR).
+
+  Lemma equivI_elim_own {A: cmra} `{Hin: inG Σ A} γ (a b: A):
+    (a ≡ b) → own γ a ⊣⊢ own γ b.
+  Proof. iIntros (Hequiv). rewrite Hequiv. eauto. Qed.
+
+  Lemma know_full_equiv ℓ abs_hist :
+    know_full_history_loc ℓ abs_hist ⊣⊢ know_full_encoded_history_loc ℓ (encode <$> abs_hist).
+  Proof.
+    apply equivI_elim_own.
+    do 3 f_equiv.
+    rewrite /abs_hist_to_ra.
+    rewrite map_fmap_compose.
+    done.
+  Qed.
+
+  Lemma abs_hist_to_ra_inj hist hist' :
+    abs_hist_to_ra hist' ≡ abs_hist_to_ra hist →
+    hist' = hist.
+  Proof.
+    intros eq.
+    apply: map_eq. intros t.
+    pose proof (eq t) as eq'.
+    rewrite !lookup_fmap in eq'.
+    destruct (hist' !! t) as [h|] eqn:leq, (hist !! t) as [h'|] eqn:leq';
+      rewrite leq leq'; rewrite leq leq' in eq'; try inversion eq'; auto.
+    simpl in eq'.
+    apply Some_equiv_inj in eq'.
+    apply to_agree_inj in eq'.
+    apply encode_inj in eq'.
+    rewrite eq'.
+    done.
+  Qed.
+
+  Lemma abs_hist_to_ra_agree hist hist' :
+    to_agree <$> hist' ≡ abs_hist_to_ra hist →
+    hist' = encode <$> hist.
+  Proof.
+    intros eq.
+    apply: map_eq. intros t.
+    pose proof (eq t) as eq'.
+    rewrite !lookup_fmap in eq'.
+    rewrite lookup_fmap.
+    destruct (hist' !! t) as [h|] eqn:leq, (hist !! t) as [h'|] eqn:leq';
+      rewrite ?leq leq'; rewrite ?leq ?leq' in eq'; try inversion eq'; auto.
+    simpl in eq'. simpl.
+    apply Some_equiv_inj in eq'.
+    apply to_agree_inj in eq'.
+    f_equiv.
+    apply eq'.
+  Qed.
+
+  (** If you know the full history for a location and own the "all-knowing"
+  resource, then those two will agree. *)
+  Lemma own_full_history_agree ℓ hist hists :
+    own_full_history hists -∗
+    know_full_history_loc ℓ hist -∗
+    ⌜hists !! ℓ = Some (encode <$> hist)⌝.
+  Proof.
+    iIntros "O K".
+    iDestruct (own_valid_2 with "O K") as %[Incl _]%auth_both_valid_discrete.
+    iPureIntro.
+    apply singleton_included_l in Incl as [encHist' [look incl]].
+    rewrite lookup_fmap in look.
+    destruct (hists !! ℓ) as [hist'|] eqn:histsLook.
+    2: { rewrite histsLook in look. inversion look. }
+    rewrite histsLook in look.
+    simpl in look.
+    apply Some_equiv_inj in look.
+    f_equiv.
+    apply abs_hist_to_ra_agree.
+    apply Some_included in incl as [eq|incl].
+    - rewrite <- eq in look.
+      apply auth_auth_inj in look as [_ eq'].
+      done.
+    - rewrite <- look in incl.
+      assert (● (to_agree <$> hist') ≼ ● (to_agree <$> hist') ⋅ ◯ (ε : gmapUR _ _)) as incl'.
+      { eexists _. reflexivity. }
+      pose proof (transitivity incl incl') as incl''.
+      apply auth_auth_included in incl''.
+      done.
+  Qed.
+
+End abs_history_lemmas.
 
 Section wpc.
   Context `{!nvmG Σ}.
+
+  (** This is our analog to the state interpretation in the Iris weakest
+  precondition. We keep this in our crash weakest precondition ensuring that it
+  holds before and after each step. **)
+  Definition interp : iProp Σ :=
+    (∃ (abs_hists : enc_abs_histories),
+      ([∗ map] ℓ ↦ abs_hist ∈ abs_hists,
+        (* We keep half the points-to predicates to ensure that we know that the
+        keys in the abstract history correspond to the physical history. This
+        ensures that on a crash we know that the value recoreved after a crash
+        has a corresponding abstract value. *)
+        ∃ (hist : history), 
+          ⌜ dom (gset _) abs_hist = dom _ hist ⌝ ∗
+          ℓ ↦h{#1/2} hist) ∗
+      (* Ownership over the full knowledge of the abstract history of _all_ locations. *)
+      own_full_history abs_hists).
 
   Program Definition wpc_def s k E e (Φ : val → dProp Σ) (Φc : dProp Σ) : dProp Σ :=
     MonPred (λ V,
@@ -36,6 +160,23 @@ Section wpc.
     rewrite wpc_eq. constructor => V. solve_proper.
   Qed.
 
+  Global Instance wpc_proper s k E1 e :
+    Proper (pointwise_relation _ (≡) ==> (≡) ==> (≡)) (wpc s k E1 e).
+  Proof.
+    rewrite wpc_eq. constructor => V. solve_proper.
+  Qed.
+
+  (** The weakest precondition is defined in terms of the crash weakest precondition. *)
+  Definition wp_def : Wp expr_lang (dProp Σ) stuckness :=
+    λ s E e Φ, (WPC e @ s ; 0 ; E {{ Φ }} {{ True }})%I.
+  Definition wp_aux : seal (@wp_def). Proof. by eexists. Qed.
+  Definition wp' := wp_aux.(unseal).
+  (* Global Arguments wp' {Λ Σ _}. *)
+  (* Check wp'. *)
+  Global Existing Instance wp'.
+  Lemma wp_eq : wp = @wp_def.
+  Proof. rewrite -wp_aux.(seal_eq) //. Qed.
+
   Lemma wpc_bind K s k E1 (e : expr) Φ Φc :
     WPC e @ s; k; E1 {{ v, WPC fill K (of_val v) @ s; k; E1 {{ Φ }} {{ Φc }} }} {{ Φc }}
                       ⊢ WPC fill K e @ s; k; E1 {{ Φ }} {{ Φc }}.
@@ -57,6 +198,71 @@ Section wpc.
     iApply (wpc_crash_mono with "[] HI").
     iModIntro.
     iIntros "$".
+  Qed.
+
+  Lemma wp_wpc s k E1 e Φ:
+    WP e @ s ; E1 {{ Φ }} ⊢ WPC e @ s ; k ; E1 {{ Φ }} {{ True }}.
+  Proof.
+    iStartProof (iProp _).
+    rewrite wp_eq /wp_def wpc_eq /wpc_def.
+    iIntros (?) "H /=". iIntros (TV ?) "??".
+    setoid_rewrite (monPred_at_pure ⊥).
+    rewrite /crash_weakestpre.wpc_def crash_weakestpre.wpc_eq.
+    iIntros (n).
+    iApply wpc0_change_k.
+    iApply ("H" $! TV with "[% //] [$] [$]").
+  Qed.
+
+  (*
+  Lemma wpc_wp s k E1 e Φ Φc:
+    WPC e @ s ; k ; E1 {{ Φ }} {{ Φc }} ⊢ WP e @ s ; E1 {{ Φ }}.
+  Proof.
+    rewrite wp_eq /wp_def wpc_eq. iIntros "H" (?).
+    iApply wpc0_change_k.
+    iApply (wpc0_strong_mono with "H"); auto. by apply omega_le_refl.
+  Qed.
+  *)
+
+  Locate "={".
+  (* uPred_fupd_level *)
+
+  Program Definition ncfupd_def `{!invG Σ, !crashG Σ} (E1 E2 : coPset) (P : dProp Σ) : dProp Σ :=
+    MonPred (λ TV, ∀ q, NC q -∗ |={E1, E2}=> (P TV) ∗ NC q)%I _.
+  Next Obligation. solve_proper. Qed.
+  Definition ncfupd_aux `{!invG Σ, !crashG Σ} : seal (ncfupd_def). Proof. by eexists. Qed.
+  Definition ncfupd `{!invG Σ, !crashG Σ} := ncfupd_aux.(unseal).
+  Definition ncfupd_eq `{!invG Σ, !crashG Σ} : ncfupd = ncfupd_def := ncfupd_aux.(seal_eq).
+
+  (* Program Definition uPred_fupd_level_def `{!invG Σ} (E1 E2 : coPset) (k : nat) (P : dProp Σ) : dProp Σ := *)
+  (*   MonPred (λ TV, uPred_fupd_split_level E1 E2 k None (P TV)) _. *)
+  (* Next Obligation. solve_proper. Qed. *)
+  (* Definition uPred_fupd_level_aux `{!invG Σ} : seal uPred_fupd_level_def. Proof. by eexists. Qed. *)
+  (* Definition uPred_fupd_level `{!invG Σ} := uPred_fupd_level_aux.(unseal). *)
+
+  (* Notation "| k ={ E1 }=> Q" := (uPred_fupd_level E1 E1 k Q) : bi_scope. *)
+  (* From Perennial.base_logic.lib Require Export ncfupd. *)
+
+  Lemma wpc_value s k E1 (Φ : val → dProp Σ) Φc (v : val) :
+    ((ncfupd_def E1 E1 (Φ v))) ∧ (<disc> |C={E1}_k=> Φc) ⊢ WPC of_val v @ s; k; E1 {{ Φ }} {{ Φc }}.
+    (* ((|NC={E1}=> Φ v) : dProp _) ∧ (<disc> |C={E1}_k=> Φc) ⊢ WPC of_val v @ s; k; E1 {{ Φ }} {{ Φc }}. *)
+  Proof.
+    rewrite wpc_unfold /wpc_pre to_of_val. iIntros "H".
+    iIntros (mj).
+    iModIntro.
+    iSplit.
+    - iDestruct "H" as "(H&_)". rewrite ncfupd_eq /ncfupd_def.
+      iIntros (q) "HNC". iMod ("H" with "HNC"). by iFrame.
+    - iDestruct "H" as "(_&H)". iIntros. iModIntro.
+      by iApply cfupd_split_level_cfupd.
+  Qed.
+
+  Lemma wpc_value' s k E1 Φ Φc v :
+  Φ v ∧ <disc> Φc ⊢ WPC of_val v @ s; k; E1 {{ Φ }} {{ Φc }}.
+  Proof.
+    iIntros "H". iApply wpc_value.
+    iSplit.
+    - iModIntro. iDestruct "H" as "($&_)".
+    - iDestruct "H" as "(_&H)". by do 2 iModIntro.
   Qed.
 
 End wpc.
