src/high/resources.v
@@ -1,0 +1,40 @@
+(* We define the resource algebras that we use in the interpretation of the
+high-level logic. *)
+From iris.base_logic.lib Require Import own.
+From iris.algebra Require Import gmap excl auth.
+
+From self.lang Require Import lang.
+From self.base Require Import primitive_laws.
+From self.high Require Import dprop.
+
+Notation st := positive (only parsing).
+Notation stO := positiveO (only parsing).
+
+Definition predicateR {Σ} := agreeR (st -d> val -d> laterO (optionO (dPropO Σ))).
+Definition predicatesR {Σ} := authR (gmapUR loc (@predicateR Σ)).
+
+Definition abs_history (State : Type) `{Countable State} := gmap time State.
+
+Definition encoded_abs_historyR := gmapUR time (agreeR stO).
+Definition enc_abs_histories := gmap loc (gmap time st).
+
+Definition abs_historiesR := authR (gmapUR loc (authR encoded_abs_historyR)).
+
+Class nvmHighG Σ := NvmHighG {
+  abs_history_name : gname;
+  predicates_name : gname;
+  ra_inG :> inG Σ (@predicatesR Σ);
+  ra'_inG :> inG Σ abs_historiesR;
+}.
+
+Class nvmG Σ := NvmG {
+  nvmG_baseG :> nvmBaseG Σ;
+  nvmG_highG :> nvmHighG Σ;
+}.
+
+Class AbstractState T := {
+  abs_state_eqdecision :> EqDecision T;
+  abs_state_countable :> Countable T;
+  abs_state_subseteq :> SqSubsetEq T;
+  abs_state_preorder :> PreOrder (⊑@{T});
+}.
